added ex 1 and 3

BoilerPlate/Ex1.dfy
@@ -12,13 +12,58 @@ function serialise<V>(t : Tree<V>) : seq<Code<V>>
   }
 }
 
-
 // Ex 1
-function deserialise<V>(cs : seq<Code<V>>) : Tree<V> 
+function deserialiseAux<T>(codes: seq<Code<T>>, trees: seq<Tree<T>>): seq<Tree<T>>
+  requires |codes| > 0 || |trees| > 0
+  ensures |deserialiseAux(codes, trees)| >= 0
+  decreases codes
 {
-  // ToDo
+  if |codes| == 0 then trees
+  else
+    match codes[0] {
+      case CLf(v) => deserialiseAux(codes[1..], trees + [Leaf(v)])
+      case CSNd(v) => if (|trees| >= 1) then deserialiseAux(codes[1..], trees[..|trees|-1] + [SingleNode(v, trees[|trees|-1])]) else trees
+      case CDNd(v) => if (|trees| >= 2) then deserialiseAux(codes[1..], trees[..|trees|-2] + [DoubleNode(v, trees[|trees|-1], trees[|trees|-2])]) else trees
+    }
 }
 
+function deserialise<T>(s:seq<Code<T>>):seq<Tree<T>>
+  requires |s| > 0
+{
+  deserialiseAux(s, [])
+}
+
+method testSerializeWithAnEmptyTree()
+{
+  var tree := Leaf(42);
+  var result := serialise(tree);
+  assert result == [CLf(42)];
+}
+
+method testSerializeNullValues()
+{
+    var tree := Leaf(null);
+    var result := serialise(tree);
+    assert result == [CLf(null)];
+}
+
+method testSerializeWithAllElements()
+{
+  var tree: Tree<int> := DoubleNode(9, Leaf(6), DoubleNode(2, Leaf(5), SingleNode(4, Leaf(3))));
+  var codes := serialise(tree);
+  assert |codes| == 6;
+  var expectedCodes := [CLf(3), CSNd(4), CLf(5), CDNd(2), CLf(6), CDNd(9)];
+  assert codes == expectedCodes;
+}
+
+method testDeserialiseWithAllElements()
+{
+    var codes: seq<Code<int>> := [CLf(3), CSNd(4), CLf(5), CDNd(2), CLf(6), CDNd(9)];
+    var trees := deserialise(codes);
+    assert |trees| == 1; 
+    var expectedTree := DoubleNode(9, Leaf(6), DoubleNode(2, Leaf(5), SingleNode(4, Leaf(3))));
+    assert trees[0] == expectedTree;
+}
 
 // Ex 2
 
@@ -26,13 +71,28 @@ function deserialise<V>(cs : seq<Code<V>>) : Tree<V>
 
 // Ex 4 
 
+/*
 lemma SerialiseLemma<V>(t : Tree<V>)
   ensures deserialise(serialise(t)) == t 
 {
   // ToDo
 }
+*/
 
-
+/*
+function deserialiseAux<T>(codes: seq<Code<T>>, trees: seq<Tree<T>>): seq<Tree<T>>
+  decreases codes
+  requires |codes| > 0 || |trees| > 0
+  ensures |deserialiseAux(codes, trees)| >= 0
+{
+  if |codes| == 0 then trees
+  else
+    if codes[0] == CLf(v) then deserialiseAux(codes[1..], trees + [Leaf(v)])
+    else if codes[0] == CSNd(v) then deserialiseAux(codes[1..], trees[..|trees|-1] + [SingleNode(v, trees[|trees|-1])])
+    else if codes[0] == CDNd(v) then deserialiseAux(codes[1..], trees[..|trees|-2] + [DoubleNode(v, trees[|trees|-1], trees[|trees|-2])])
+    else trees
+}
+*/
 
 
 
