BoilerPlate/Ex3.dfy
@@ -52,10 +52,25 @@ class Node {
 
 
   // Ex1
-  method reverse(tail : Node?) returns (r : Node) 
+  method reverse(tail : Node?) returns (r : Node)
+    requires this.Valid()
+    requires tail != null ==> tail.Valid()
+    ensures this.next != null ==> this.list == [this.data] + this.next.list
+    ensures this.Valid()
+    ensures r.Valid()
+    ensures r.list == reverseList(old(this.list))
+    ensures this.next != null ==> this.next.footprint >= old(this.footprint)
+    decreases this.footprint
   {
     var old_next := this.next; 
-    this.next := tail; 
+    this.next := tail;
+    if (this.next == null) {
+      this.list := [this.data];
+      this.footprint := { this };
+    } else {
+      this.list := [this.data] + tail.list;
+      this.footprint := {this} + tail.footprint;
+    }
     
     if (old_next == null) {
       r := this; 
@@ -66,14 +81,28 @@ class Node {
     }
   }
 
+  function reverseList(lst: seq<int>) : (reversed: seq<int>)
+  decreases |lst|
+  {
+    if (lst == []) then []
+    else (reverseList(lst[1..]) + [lst[0]])
+  }
 }
 
-
-// Ex2
-
-method ExtendList(lst : Node?, v : int) returns (r : Node) 
-{
-  // ToDo 
-}
-
+  // Ex2
+  method ExtendList(nd : Node?, v : int) returns (r : Node)
+    //requires nd != null ==> v !in nd.list
+    requires nd != null ==> nd.Valid()
+    ensures r.Valid()
+    ensures fresh(r)
+  {
+    if (nd == null) {
+      r := new Node(v);
+      return;
+    }
+    else {
+      r := nd.prepend(v);
+      return;
+    }
+  }
 }
